code/ecdsap256/Hacl.Impl.P256.Point.fst
@@ -52,7 +52,7 @@ let create_aff_point () =
 
 (* https://crypto.stackexchange.com/questions/43869/point-at-infinity-and-error-handling*)
 val lemma_mont_is_point_at_inf: p:S.jacob_point{let (_, _, z) = p in z < S.prime} ->
-  Lemma (S.is_point_at_inf p == S.is_point_at_inf (SM.from_mont_point p))
+  Lemma (S.is_point_at_inf p == S.is_point_at_inf (from_mont_point p))
 
 let lemma_mont_is_point_at_inf p =
   let px, py, pz = p in
@@ -136,7 +136,7 @@ val norm_jacob_point_z: p:point -> res:felem -> Stack unit
     live h res /\ live h p /\ disjoint p res /\
     point_inv h p)
   (ensures fun h0 _ h1 -> modifies (loc res) h0 h1 /\
-    (let _, _, rz = S.norm_jacob_point (SM.from_mont_point (as_point_nat h0 p)) in
+    (let _, _, rz = S.norm_jacob_point (from_mont_point (as_point_nat h0 p)) in
     as_nat h1 res == rz))
 
 let norm_jacob_point_z p res =
@@ -176,7 +176,7 @@ val norm_jacob_point_y: p:point -> res:felem -> Stack unit
     live h res /\ live h p /\ disjoint p res /\
     point_inv h p)
   (ensures fun h0 _ h1 -> modifies (loc res) h0 h1 /\
-    (let _, ry, _ = S.norm_jacob_point (SM.from_mont_point (as_point_nat h0 p)) in
+    (let _, ry, _ = S.norm_jacob_point (from_mont_point (as_point_nat h0 p)) in
     as_nat h1 res == ry))
 
 let norm_jacob_point_y p res =
